@prefix rdf: <http://www.w3.org/1999/02/22-rdf-syntax-ns#> .
@prefix rdfs: <http://www.w3.org/2000/01/rdf-schema#> .
@prefix xsd: <http://www.w3.org/2001/XMLSchema#> .
@prefix owl: <http://www.w3.org/2002/07/owl#> .
@prefix xdd: <http://terminusdb.com/schema/xdd#> .
@prefix terminus: <http://terminusdb.com/schema/terminus#> .
@prefix layer: <http://terminusdb.com/schema/layer#> .

<http://terminusdb.com/schema/terminus>
  a owl:Ontology ;
  rdfs:label "Terminus DB Management Schema"@en ;
  rdfs:comment "Schema describing all of the structure of the documents (capabilities, roles, resources, users, databases) in the capability database used by Terminus DB to manage the internal state of the server and the databases it manages"@en ;
  terminus:rights "Copyright Data Chemist Ltd. 2017-2019"@en ;
  terminus:author "Gavin Mendel-Gleason"@en, "Kevin C. Feeney"@en ;
  terminus:license <https://creativecommons.org/licenses/by-sa/2.0/>, <https://www.gnu.org/licenses/gpl-3.0.en.html> .

terminus:Document
  a owl:Class ;
  terminus:tag terminus:abstract ;
  rdfs:label "Document Class"@en ;
  rdfs:comment "A class used to designate the primary data objects managed by the system - relationships and entities"@en .

terminus:Agent
  rdfs:label "Agent"@en ;
  rdfs:comment "An agent is an abstraction of a thing that can have a capability"@en ;
  a owl:Class ;
  terminus:tag terminus:abstract ;
  rdfs:subClassOf terminus:Document .

terminus:rights
  a owl:DatatypeProperty ;
  rdfs:range xsd:string ;
  rdfs:domain owl:Ontology ;
  rdfs:label "Rights"@en ;
  rdfs:comment "The statement of rights of the owner"@en .

terminus:author
  a owl:DatatypeProperty ;
  rdfs:domain owl:Ontology ;
  rdfs:range xsd:string ;
  rdfs:label "Author"@en ;
  rdfs:comment "The authors who developed the ontology"@en .

terminus:license
  a owl:ObjectProperty ;
  rdfs:domain owl:Ontology ;
  rdfs:range owl:Thing ;
  rdfs:label "License"@en ;
  rdfs:comment "The license governing the use of the resource"@en .

terminus:authority
  rdfs:label "Has Capability"@en ;
  rdfs:comment "A property that links an agent to a capability that they possess"@en ;
  a owl:ObjectProperty ;
  rdfs:domain terminus:Agent ;
  rdfs:range terminus:Capability .

terminus:Role
  rdfs:label "Role"@en ;
  rdfs:comment "A role is a collection of capabilities that can be allocated to any user"@en ;
  a owl:Class ;
  rdfs:subClassOf terminus:Agent .

terminus:User
  rdfs:label "User"@en ;
  rdfs:comment "A user of the database"@en ;
  a owl:Class ;
  rdfs:subClassOf terminus:Agent .

terminus:email
  rdfs:label "Email Address"@en ;
  rdfs:comment "A email address that allows the user to be contacted outside the system"@en ;
  a owl:DatatypeProperty ;
  rdfs:domain terminus:User ;
  rdfs:range xdd:email .

terminus:Capability
  a owl:Class ;
  rdfs:subClassOf terminus:Document ;
  rdfs:label "Capability"@en ;
  rdfs:comment "A capability confers access to a database or server action"@en .

terminus:Access
  a owl:Class ;
  rdfs:label "Access"@en ;
  rdfs:comment "Access actions and scopes"@en .

terminus:access
  a owl:ObjectProperty ;
  rdfs:label "access"@en ;
  rdfs:comment "associates a capability with its access patterns"@en ;
  rdfs:domain terminus:Capability ;
  rdfs:range terminus:Access .

terminus:authority_scope
  a owl:ObjectProperty ;
  rdfs:label "Capability Scope"@en ;
  rdfs:comment "The scope of the access - the resource that the capability applies to"@en ;
  rdfs:domain terminus:Access ;
  rdfs:range terminus:Resource .

terminus:resource_includes
  rdfs:label "Resource Inclusion"@en ;
  rdfs:comment "Resource A includes Resource B if A resource_includes B i.e. A Server might include a Database within its scope"@en ;
  a owl:ObjectProperty ;
  rdfs:domain terminus:Resource ;
  rdfs:range terminus:Resource .

terminus:action
  rdfs:label "Action"@en ;
  rdfs:comment "Refers to a specific API access call"@en ;
  a owl:ObjectProperty ;
  rdfs:domain terminus:Access ;
  rdfs:range terminus:DBAction .

terminus:DBAction
  rdfs:label "DB Action"@en ;
  a owl:Class ;
  owl:oneOf (
    terminus:create_database
    terminus:delete_database
    terminus:class_frame
    terminus:clone
    terminus:fetch
    terminus:push
    terminus:branch
    terminus:rebase
    terminus:instance_read_access
    terminus:instance_write_access
    terminus:schema_read_access
    terminus:schema_write_access
    terminus:inference_read_access
    terminus:inference_write_access
    terminus:meta_read_access
    terminus:meta_write_access
    terminus:commit_read_access
    terminus:commit_write_access
    terminus:manage
    ).

terminus:delete_database
  rdfs:label "Delete Database"@en ;
  rdfs:comment "An action that deletes an entire database"@en ;
  a terminus:DBAction.

terminus:schema_write_access
  rdfs:label "Update Schema"@en ;
  rdfs:comment "An action that updates the DB schema"@en ;
  a terminus:DBAction.

terminus:schema_read_access
  rdfs:label "Get Schema"@en ;
  rdfs:comment "An action that fetches the DB Schema"@en ;
  a terminus:DBAction.

terminus:inference_write_access
  rdfs:label "Update Inference"@en ;
  rdfs:comment "An action that updates the DB inference"@en ;
  a terminus:DBAction.

terminus:inference_read_access
  rdfs:label "Get Inference"@en ;
  rdfs:comment "An action that fetches the DB Inference"@en ;
  a terminus:DBAction.

terminus:class_frame
  rdfs:label "Class Frame"@en ;
  rdfs:comment "An action that fetches a Frame JSON for the appropriate Class"@en ;
  a terminus:DBAction.

terminus:create_database
  rdfs:label "Create Database"@en ;
  rdfs:comment "An action which creates a new database"@en ;
  a terminus:DBAction.

terminus:clone
  rdfs:label "Clone"@en ;
  rdfs:comment "An action which represents cloning a database"@en ;
  a terminus:DBAction .

terminus:fetch
  rdfs:label "Fetch"@en ;
  rdfs:comment "An action which represents fetching a database from a remote origin"@en ;
  a terminus:DBAction .

terminus:push
  rdfs:label "Push"@en ;
  rdfs:comment "An action which represents pushing a database to a remote origin"@en ;
  a terminus:DBAction .

terminus:branch
  rdfs:label "Branch"@en ;
  rdfs:comment "An action which represents creating a new branch of a database"@en ;
  a terminus:DBAction .

terminus:rebase
  rdfs:label "Rebase"@en ;
  rdfs:comment "An action which represents Rebasing a database branch"@en ;
  a terminus:DBAction .

terminus:instance_read_access
  rdfs:label "Instance Read Access"@en ;
  rdfs:comment "An action which allows all read-only instance data accesses to the database"@en ;
  a terminus:DBAction .

terminus:instance_write_access
  rdfs:label "Instance Write Access"@en ;
  rdfs:comment "An action which allows all write instance data accesses to the database"@en ;
  a terminus:DBAction .

terminus:schema_read_access
  rdfs:label "Schema Read Access"@en ;
  rdfs:comment "An action which allows all read-only schema data accesses to the database"@en ;
  a terminus:DBAction .

terminus:schema_write_access
  rdfs:label "Schema Write Access"@en ;
  rdfs:comment "An action which allows all write schema data accesses to the database"@en ;
  a terminus:DBAction .

terminus:inference_read_access
  rdfs:label "Inference Read Access"@en ;
  rdfs:comment "An action which allows all read-only inference data accesses to the database"@en ;
  a terminus:DBAction .

terminus:inference_write_access
  rdfs:label "Inference Write Access"@en ;
  rdfs:comment "An action which allows all write inference data accesses to the database"@en ;
  a terminus:DBAction .

terminus:meta_read_access
  rdfs:label "Meta Read Access"@en ;
  rdfs:comment "An action which allows all read-only meta data accesses to the database"@en ;
  a terminus:DBAction .

terminus:meta_write_access
  rdfs:label "Meta Write Access"@en ;
  rdfs:comment "An action which allows meta data write accesses to the database"@en ;
  a terminus:DBAction .

terminus:commit_read_access
  rdfs:label "Commit Read Access"@en ;
  rdfs:comment "An action which allows all read-only commit data accesses to the database"@en ;
  a terminus:DBAction .

terminus:commit_write_access
  rdfs:label "Commit Write Access"@en ;
  rdfs:comment "An action which allows commit data write accesses to the database"@en ;
  a terminus:DBAction .

terminus:manage
  rdfs:label "Management Access"@en ;
  rdfs:comment "An action which allows a user to manage a given database (add users, change meta-data)"@en ;
  a terminus:DBAction .

terminus:Resource
  rdfs:label "Resource"@en ;
  rdfs:comment "A resource is a thing that can be accessed and given instructions and for which capabilities can be allocated"@en ;
  a owl:Class ;
  terminus:tag terminus:abstract ;
  rdfs:subClassOf terminus:Document .

terminus:Database
  rdfs:label "Database"@en ;
  rdfs:comment "A resource representing a database hosted on the server."@en ;
  a owl:Class ;
  rdfs:subClassOf terminus:Resource .

terminus:resource_name
  rdfs:label "Resource Name"@en ;
  rdfs:comment "The resource name which is used as an internal local reference."@en ;
  a owl:DatatypeProperty ;
  rdfs:range xsd:string ;
  rdfs:domain terminus:Resource .

terminus:finalized
  a terminus:DatabaseState ;
  rdfs:label "Finalized"@en ;
  rdfs:comment "The database has been fully constructed"@en .

terminus:deleting
  a terminus:DatabaseState ;
  rdfs:label "Deleting"@en ;
  rdfs:comment "TerminusDB is in the process of deleting your database"@en .

terminus:DatabaseState
  rdfs:label "Database State"@en ;
  rdfs:comment "Class for keeping information about the state of a database." ;
  a owl:Class ;
  owl:oneOf ( terminus:finalized terminus:deleting ) .

terminus:database_state
  rdfs:label "State"@en ;
  rdfs:comment "The databases current state"@en ;
  a owl:ObjectProperty ;
  rdfs:range terminus:DatabaseState ;
  rdfs:domain terminus:Database .

terminus:allow_origin
  rdfs:label "Allow Requests from"@en ;
  rdfs:comment "Specify which domains can access this database from the web. Set to \"*\" for universal access. Sets the HTTP Access-Control-Allow-Origin header. "@en ;
  a owl:DatatypeProperty;
  rdfs:domain terminus:Resource;
  rdfs:range xsd:string.

terminus:server
  a terminus:Server ;
  rdfs:label "server"@en .

terminus:Server
  rdfs:label "Server"@en ;
  rdfs:comment "A Resource Object Representing the Database Server itself"@en ;
  a owl:Class ;
  owl:oneOf (terminus:server) ;
  rdfs:subClassOf terminus:Resource .

terminus:agent_name
  a owl:DatatypeProperty ;
  rdfs:label "Agent name"@en ;
  rdfs:comment "An name for API authentication"@en ;
  rdfs:domain terminus:Agent ;
  rdfs:range xsd:string .

terminus:agent_key_hash
  a owl:DatatypeProperty ;
  rdfs:label "Agent Key"@en ;
  rdfs:comment "An agent key for API authentication"@en ;
  rdfs:domain terminus:Agent ;
  rdfs:range xsd:string.

terminus:user_key_hash
  a owl:DatatypeProperty ;
  rdfs:label "User Key"@en ;
  rdfs:comment "A user key for API authentication"@en ;
  rdfs:domain terminus:User ;
  rdfs:range xsd:string .

terminus:prefixes
  a owl:ObjectProperty ;
  rdfs:domain terminus:Database ;
  rdfs:range terminus:Prefix ;
  rdfs:label "prefixes"@en ;
  rdfs:comment "Associates a database with its default prefixes"@en .

terminus:PrefixRestriction
  a owl:Restriction ;
  rdfs:label "Prefix Restriction"@en ;
  rdfs:comment "Only one prefix per object"@en ;
  rdfs:onProperty terminus:prefix ;
  owl:cardinality "1"^^xsd:nonNegativeInteger .

terminus:PrefixURIRestriction
  a owl:Restriction ;
  rdfs:label "Prefix URI Restriction"@en ;
  rdfs:comment "Only one prefix URI per object"@en ;
  rdfs:onProperty terminus:prefix_uri ;
  owl:cardinality "1"^^xsd:nonNegativeInteger .

terminus:Prefix
  a owl:Class ;
  rdfs:subClassOf terminus:PrefixRestriction, terminus:PrefixURIRestriction ;
  rdfs:label "Prefixes"@en ;
  rdfs:comment "Default prefixes for a given database"@en .

terminus:prefix
  a owl:DatatypeProperty ;
  rdfs:label "prefix"@en ;
  rdfs:comment "The shorthand for the initial segment of an IRI"@en ;
  rdfs:domain terminus:Prefix ;
  rdfs:range xsd:string .

terminus:prefix_uri
  a owl:DatatypeProperty ;
  rdfs:label "prefix uri"@en ;
  rdfs:comment "The uri associated with a shorthand"@en ;
  rdfs:domain terminus:Prefix ;
  rdfs:range xsd:string .
